Coherence/DelocationAlgo.v
@@ -4,7 +4,6 @@ Require Import Annotation Liveness Coherence Delocation.
 
 Set Implicit Arguments.
 Unset Printing Abstraction Types.
-Local Arguments lminus {X} {H} s L.
 
 Definition addParam x (DL:list (set var)) (AP:list (set var)) :=
   zip (fun (DL:set var) AP => if [x ∈ DL]
@@ -22,7 +21,7 @@ Qed.
 Lemma addParam_zip_lminus_length DL ZL AP x
 : length AP = length DL
   -> length DL = length ZL
-  -> length (addParam x (zip lminus DL ZL) AP) = length DL.
+  -> length (addParam x (DL \\ ZL) AP) = length DL.
 Proof.
   eauto with len.
 Qed.
@@ -48,7 +47,7 @@ Fixpoint computeParameters (DL: list (set var)) (ZL:list (list var)) (AP:list (s
       let (ar, r) := computeParameters DL ZL (addParam x DL AP) s an in
       (ann1 nil ar, r)
     | stmtFun F t, annF lv ans ant =>
-      let DL' := zip lminus (getAnn ⊝ ans) (fst ⊝ F) in
+      let DL' := (getAnn ⊝ ans) \\ (fst ⊝ F) in
       let Z : list params := List.map fst F in
       let Zset := list_union (fst ∘ of_list ⊝ F) in
       let AP' := ((fun _ => ∅) ⊝ F ++ AP) in
@@ -65,11 +64,12 @@ Fixpoint computeParameters (DL: list (set var)) (ZL:list (list var)) (AP:list (s
     | s, a => (ann0 nil, nil)
   end.
 
-Notation "'computeParametersF' DL ZL AP F als" :=
-  ((fun Zs a0 => computeParameters ((getAnn ⊝ als) \\ (fst ⊝ F) ++ DL \\ ZL)
-                                    (fst ⊝ F ++ ZL)
-                                    (List.map (fun _ => ∅) F ++ AP)
-                                    (snd Zs) a0)
+Notation "'computeParametersF' F als DL ZL AP" :=
+  ((fun Zs a0 => computeParameters
+                ((getAnn ⊝ als ++ DL) \\ ((fst ⊝ F) ++ ZL))
+                ((fst ⊝ F) ++ ZL)
+                (List.map (fun _ => ∅) F ++ AP)
+                (snd Zs) a0)
      ⊜ F als)
     (at level 50, DL, ZL, AP, F, als at level 0).
 
@@ -99,59 +99,63 @@ Local Ltac lnorm :=
           | [ |- context [ zip _ _ _ ++ zip _ _ _ ] ] => rewrite <- zip_app; [| eauto with len]
           end).
 
-Lemma computeParameters_length s lv DL ZL AP an' LV
- : computeParameters (zip lminus DL ZL) ZL AP s lv = (an', LV)
-   -> live_sound Imperative (zip pair DL ZL) s lv
-   -> length AP = length DL
-   -> length DL = length ZL
-   -> length LV = length DL.
+Lemma computeParameters_length AP s lv DL ZL
+  : live_sound Imperative ZL DL s lv
+    -> length AP = length DL
+    -> length DL = length ZL
+    -> length (snd (computeParameters (DL \\ ZL) ZL AP s lv)) = length DL.
 Proof.
-  intros CPEQ LS LEQ LEQ2 .
-  general induction LS; simpl in *; repeat let_case_eq; inv CPEQ.
-  - rewrite LEQ. eapply IHLS; eauto. rewrite addParam_zip_lminus_length; eauto.
-  - exploit IHLS1; eauto.
-    exploit IHLS2; eauto.
-    repeat rewrite zip_length2; eauto with len.
+  intros LS. revert AP.
+  induction LS; simpl in *; intros; repeat let_pair_case_eq; subst; simpl.
+  - eapply IHLS; eauto. rewrite addParam_zip_lminus_length; eauto.
+  - rewrite zip_length2; eauto.
+    rewrite IHLS1; eauto.
+    rewrite IHLS2; eauto.
   - eauto with len.
   - eauto with len.
-  - rewrite LEQ. eapply IHLS; eauto with len.
-  - lnorm.
-    exploit IHLS; eauto using live_globals_zip.
-    + eauto with len.
-    + eauto with len.
-    + rewrite length_drop_minus.
-      rewrite zip_length2.
+  - eapply IHLS; eauto with len.
+  - rewrite length_drop_minus.
+    rewrite zip_length2; eauto with len.
+    + rewrite app_length.
       repeat rewrite zip_length2; eauto with len.
-      rewrite app_length.
       rewrite map_length. omega.
-      rewrite fold_zip_ounion_length.
-      * rewrite H4. eauto with len.
-      * intros. rewrite H4. rewrite app_length, map_length.
-        rewrite <- LEQ, <- H.
-        intros. inv_map H5.
-        destruct x as [an LV]. inv_zip H6. simpl.
-        eapply H1 in H9; eauto 20 using pair_eta, live_globals_zip with len.
-        rewrite H9. eauto with len.
+    + rewrite fold_zip_ounion_length.
+      * rewrite <- zip_app; [|eauto with len].
+        rewrite IHLS; eauto with len.
+      * intros; inv_get.
+        rewrite <- zip_app; [| eauto with len].
+        rewrite IHLS; [ | eauto with len | eauto with len].
+        erewrite H1; eauto with len.
 Qed.
 
 Local Create HintDb rew.
 Local Hint Extern 20 => rewrite <- zip_app : rew.
 Local Hint Extern 20 => rewrite <- live_globals_zip; eauto with len : rew.
 
-Lemma computeParametersF_length DL ZL AP F als k
+Lemma computeParametersF_length AP (ZL:list params) (Lv: list (set var)) F als k
   : (forall n Zs a, get F n Zs -> get als n a ->
-               live_sound Imperative (pair ⊜ (getAnn ⊝ als) (fst ⊝ F) ++ pair ⊜ DL ZL) (snd Zs) a)
-    -> k = ❬getAnn ⊝ als ++ DL❭
+               live_sound Imperative (fst ⊝ F ++ ZL) (getAnn ⊝ als ++ Lv) (snd Zs) a)
+    -> k = ❬getAnn ⊝ als ++ Lv❭
     -> length F = length als
-    -> length AP = length DL
-    -> length DL = length ZL
-    -> forall n a, get (snd ⊝ computeParametersF DL ZL AP F als) n a -> k = ❬a❭.
+    -> length AP = length Lv
+    -> length Lv = length ZL
+    -> forall n a, get (snd ⊝ computeParametersF F als Lv ZL AP) n a -> ❬a❭ = k.
 Proof.
-  intros LIVE LEN1 LEN2 LEN3 n a GET. subst.
-  rewrite live_globals_zip in LIVE; eauto.
-  intros. inv_get.
-  symmetry. rewrite <- zip_app; eauto with len.
-  eapply computeParameters_length; eauto using pair_eta with len.
+  intros LIVE EQ LEN1 LEN2 LEN3 n a GET. subst.
+  inv_get. rewrite computeParameters_length; eauto with len.
+Qed.
+
+Lemma computeParametersF_length_pair AP (ZL:list params) (Lv: list (set var)) F als k
+  : (forall n Zs a, get F n Zs -> get als n a ->
+               live_sound Imperative (fst ⊝ F ++ ZL) (getAnn ⊝ als ++ Lv) (snd Zs) a)
+    -> k = ❬getAnn ⊝ als ++ Lv❭
+    -> length F = length als
+    -> length AP = length Lv
+    -> length Lv = length ZL
+    -> forall n a, get (computeParametersF F als Lv ZL AP) n a -> ❬snd a❭ = k.
+Proof.
+  intros LIVE EQ LEN1 LEN2 LEN3 n a GET. subst.
+  inv_get. rewrite computeParameters_length; eauto with len.
 Qed.
 
 Lemma ifSndR_zip_addAdd s DL A B
@@ -196,39 +200,39 @@ Proof.
   - cases; eauto using PIR2, @ifSndR.
 Qed.
 
-Lemma computeParameters_AP_LV DL ZL AP s lv an' LV
-:live_sound Imperative (zip pair DL ZL) s lv
-  -> computeParameters (zip lminus DL ZL) ZL AP s lv = (an', LV)
-  -> length AP = length DL
-  -> length DL = length ZL
-  -> PIR2 (ifSndR Subset) AP LV.
+Lemma computeParameters_AP_LV Lv ZL AP s lv
+:live_sound Imperative ZL Lv s lv
+  -> length AP = length Lv
+  -> length Lv = length ZL
+  -> PIR2 (ifSndR Subset) AP (snd (computeParameters (Lv \\ ZL) ZL AP s lv)).
 Proof.
-  intros LS CPEQ LEQ.
-  general induction LS; simpl in * |- *; repeat let_case_eq; invc CPEQ.
-  - exploit IHLS; eauto using addParam_zip_lminus_length.
-    eauto using PIR2_ifSndR_Subset_left, PIR2_addParam with len.
+  intros LS. revert AP.
+  induction LS; simpl in * |- *; intros; repeat let_pair_case_eq; subst; simpl.
+  - eapply PIR2_ifSndR_Subset_left; eauto.
+    eapply IHLS; eauto with len.
+    eapply PIR2_addParam; eauto with len.
   - eauto using ifSndR_zip_ounion.
   - eauto using PIR2_ifSndR_keep.
-  - clear_all. unfold mapi. generalize 0.
-    general induction AP; simpl; eauto using PIR2, @ifSndR.
-  - exploit IHLS; eauto using addParam_zip_lminus_length.
-    eauto using PIR2_ifSndR_Subset_left, PIR2_addParam with len.
-  - lnorm.
-    assert (APEQ: AP = drop ❬F❭ (tab {} ‖F‖ ++ AP))
-      by (rewrite drop_length_ass; eauto with len).
-    rewrite APEQ at 1. eapply PIR2_drop.
-    exploit computeParameters_length as B0LEN; eauto.
-    eauto with len. eauto with len.
-    eapply ifSndR_zip_addAdd. eauto 20 with len.
+  - eapply PIR2_get; eauto with len.
+    intros; inv_get; eauto using @ifSndR.
+  - eapply PIR2_ifSndR_Subset_left.
+    eapply IHLS; eauto using addParam_zip_lminus_length.
+    eauto using PIR2_addParam with len.
+  - rewrite <- zip_app; eauto.
+    eapply PIR2_ifSndR_Subset_left.
+    eapply PIR2_drop.
+    eapply ifSndR_zip_addAdd.
+    Focus 2.
     eapply ifSndR_fold_zip_ounion; eauto.
+    Focus 2.
+    eapply IHLS; eauto with len.
     + clear IHLS. intros.
       inv_get.
       eapply H1;
-      eauto using PIR2_drop, live_globals_zip, pair_eta with len rew.
-    + exploit IHLS; [ eauto
-                    | eauto with len
-                    | eapply eq
-                    | | | ]; eauto 20 with len.
+        eauto using PIR2_drop, live_globals_zip, pair_eta with len rew.
+    + eauto 20 with len.
+    + rewrite drop_length_ass; eauto with len.
+    + eauto with len.
 Qed.
 
 Lemma ifFstR_addAdds s A B
@@ -265,34 +269,31 @@ Proof.
   eapply PIR2_get; try (intros ? ? ? GET; inv_map GET); eauto with cset len.
 Qed.
 
-Lemma computeParameters_LV_DL DL ZL AP s lv an' LV
-: live_sound Imperative (zip pair DL ZL) s lv
-  -> computeParameters (zip lminus DL ZL) ZL AP s lv = (an', LV)
-  -> length AP = length DL
-  -> length DL = length ZL
-  -> PIR2 Subset AP (zip lminus DL ZL)
-  -> PIR2 (ifFstR Subset) LV (zip lminus DL ZL).
+Lemma computeParameters_LV_DL ZL Lv AP s lv
+: live_sound Imperative ZL Lv s lv
+  -> length AP = length Lv
+  -> length Lv = length ZL
+  -> PIR2 Subset AP (Lv \\ ZL)
+  -> PIR2 (ifFstR Subset) (snd (computeParameters (Lv \\ ZL) ZL AP s lv)) (Lv \\ ZL).
 Proof.
-  intros LS CPEQ LEQ.
-  general induction LS; simpl in * |- *; repeat let_case_eq; invc CPEQ.
-  - exploit IHLS; eauto using addParam_zip_lminus_length.
-    eapply addParam_Subset; eauto.
+  intros LS Len1 Len2 LEQ.
+  general induction LS; simpl in * |- *; repeat let_pair_case_eq; subst; simpl.
+  - eapply IHLS; eauto using addParam_Subset with len.
   - eauto using ifFstR_zip_ounion.
   - eauto using PIR2_ifFstR_Subset_right, PIR2_ifFstR_keep.
   - eapply PIR2_get; eauto with len.
     intros. inv_get; econstructor.
-  - exploit IHLS; eauto using addParam_zip_lminus_length.
-    eapply addParam_Subset; eauto.
-  - assert (EQ: DL \\ ZL = drop ❬F❭ ((getAnn ⊝ als) \\ (fst ⊝ F) ++ DL \\ ZL))
+  - eapply IHLS; eauto using addParam_zip_lminus_length, addParam_Subset.
+  - assert (EQ: Lv \\ ZL = drop ❬F❭ ((getAnn ⊝ als) \\ (fst ⊝ F) ++ Lv \\ ZL))
       by (rewrite drop_length_ass; eauto with len).
-    rewrite EQ at 2.
+    rewrite EQ at 4.
     lnorm.
     eapply PIR2_drop.
     eapply ifFstR_addAdds; eauto.
     eapply ifFstR_fold_zip_ounion; eauto.
     + intros ? ? GET. inv_get.
-      eapply H1; eauto using pair_eta, live_globals_zip, PIR2_Subset_tab_extend with len.
-    + eapply IHLS; eauto 20 using pair_eta, live_globals_zip, PIR2_Subset_tab_extend with len.
+      eapply H1; eauto using PIR2_Subset_tab_extend with len.
+    + eapply IHLS; eauto 20 using PIR2_Subset_tab_extend with len.
 Qed.
 
 Lemma PIR2_olist_union_bound X `{OrderedType X} A b c
@@ -304,53 +305,52 @@ Proof.
   - eapply IHA; eauto using get, ifFstR_zip_ounion.
 Qed.
 
-Lemma computeParametersF_LV_DL DL ZL AP F als A
+Lemma computeParametersF_LV_DL ZL Lv AP F als A
 : (forall n Zs a, get F n Zs -> get als n a ->
-            live_sound Imperative (pair ⊜ (getAnn ⊝ als) (fst ⊝ F) ++ pair ⊜ DL ZL) (snd Zs) a)
-  -> PIR2 Subset AP (zip lminus DL ZL)
-  -> PIR2 (ifFstR Subset) A ((getAnn ⊝ als ++ DL) \\ (fst ⊝ F ++ ZL))
-  -> length AP = length DL
-  -> length DL = length ZL
+            live_sound Imperative (fst ⊝ F ++ ZL) (getAnn ⊝ als ++ Lv) (snd Zs) a)
+  -> PIR2 Subset AP (Lv \\ ZL)
+  -> PIR2 (ifFstR Subset) A ((getAnn ⊝ als ++ Lv) \\ (fst ⊝ F ++ ZL))
+  -> length AP = length Lv
+  -> length Lv = length ZL
   -> length F = length als
-  -> PIR2 (ifFstR Subset) (olist_union (snd ⊝ computeParametersF DL ZL AP F als) A)
-         ((getAnn ⊝ als ++ DL) \\ (fst ⊝ F ++ ZL)).
+  -> PIR2 (ifFstR Subset) (olist_union (snd ⊝ computeParametersF F als Lv ZL AP) A)
+         ((getAnn ⊝ als ++ Lv) \\ (fst ⊝ F ++ ZL)).
 Proof.
   intros. eapply PIR2_olist_union_bound; eauto.
-  intros. inv_get. rewrite <- zip_app in H; eauto with len.
-  rewrite <- zip_app; eauto with len.
-  eapply computeParameters_LV_DL; eauto using pair_eta, PIR2_Subset_tab_extend with len.
+  intros; inv_get.
+  eapply computeParameters_LV_DL; eauto using PIR2_Subset_tab_extend with len.
 Qed.
 
 Lemma get_olist_union_b X `{OrderedType X} A b n x
   : get b n (Some x)
-    -> (forall n a, get A n a -> ❬b❭ = ❬a❭)
+    -> (forall n a, get A n a -> ❬a❭ = ❬b❭)
     -> exists s, get (olist_union A b) n (Some s) /\ x ⊆ s.
 Proof.
   intros GETb LEN. general induction A; simpl in *.
   - eexists x. eauto with cset.
   - exploit LEN; eauto using get.
-    edestruct (get_length_eq _ GETb H0) as [y GETa]; eauto.
+    edestruct (get_length_eq _ GETb (eq_sym H0)) as [y GETa]; eauto.
     exploit (zip_get ounion GETb GETa).
     destruct y; simpl in *.
-    exploit IHA; try eapply GET; eauto.
-    rewrite zip_length2; eauto using get with len.
-    edestruct H2; dcr; subst. eexists; split; eauto.
-    rewrite <- H7; eauto.
-    exploit IHA; try eapply GET; eauto.
-    rewrite zip_length2; eauto using get with len.
+    + exploit IHA; try eapply GET; eauto.
+      rewrite zip_length2; eauto using get with len.
+      edestruct H2; dcr; subst. eexists; split; eauto.
+      rewrite <- H7; eauto.
+    + exploit IHA; try eapply GET; eauto.
+      rewrite zip_length2; eauto using get with len.
 Qed.
 
 Lemma get_olist_union_A X `{OrderedType X} A a b n k x
   : get A k a
     -> get a n (Some x)
-    -> (forall n a, get A n a -> ❬b❭ = ❬a❭)
+    -> (forall n a, get A n a -> ❬a❭ = ❬b❭)
     -> exists s, get (olist_union A b) n (Some s) /\ x ⊆ s.
 Proof.
   intros GETA GETa LEN.
   general induction A; simpl in * |- *; isabsurd.
   inv GETA; eauto.
   - exploit LEN; eauto using get.
-    edestruct (get_length_eq _ GETa (eq_sym H0)) as [y GETb].
+    edestruct (get_length_eq _ GETa H0) as [y GETb].
     exploit (zip_get ounion GETb GETa).
     destruct y; simpl in *.
     exploit (@get_olist_union_b _ _ A); eauto.
@@ -363,146 +363,162 @@ Proof.
     rewrite zip_length2; eauto using get with len.
 Qed.
 
+Lemma get_olist_union_A' X `{OrderedType X} A a b n k x p
+  : get A k a
+    -> get a n (Some x)
+    -> (forall n a, get A n a -> ❬a❭ = ❬b❭)
+    -> get (olist_union A b) n p
+    -> exists s, p = (Some s) /\ x ⊆ s.
+Proof.
+  intros. edestruct get_olist_union_A; eauto; dcr.
+  get_functional; eauto.
+Qed.
+
 Tactic Notation "Rexploit" uconstr(H) :=
   eapply modus_ponens; [refine H | intros].
 
 Tactic Notation "Rexploit" uconstr(X) "as" ident(H)  :=
   eapply modus_ponens; [refine X | intros H].
 
-Lemma computeParameters_isCalled_Some DL ZL AP s lv an' LV n D Z p
-: live_sound Imperative (zip pair DL ZL) s lv
-  -> computeParameters (zip lminus DL ZL) ZL AP s lv = (an', LV)
-  -> length AP = length DL
-  -> length DL = length ZL
+Lemma computeParameters_isCalled_Some ZL Lv AP s lv n D Z p
+: live_sound Imperative ZL Lv s lv
+  -> length AP = length Lv
+  -> length Lv = length ZL
   -> isCalled s (LabI n)
-  -> get DL n D
+  -> get Lv n D
   -> get ZL n Z
-  -> get LV n p
+  -> get (snd (computeParameters (Lv \\ ZL) ZL AP s lv)) n p
   -> exists Za, p = Some Za /\ D \ of_list Z \ Za ⊆ (getAnn lv).
 Proof.
-  intros LS CPEQ LEN1 LEN2 IC GetDL GetZL GetLV.
-  general induction IC; simpl in * |- *; inv LS; repeat let_case_eq; invc CPEQ.
-  - edestruct IHIC as [Za [A B]]; eauto with len. subst; simpl.
+  intros LS LEN1 LEN2 IC GetDL GetZL GetLV.
+  general induction IC; simpl in * |- *; inv LS;
+    repeat let_case_eq; repeat let_pair_case_eq; subst; simpl in *.
+  - edestruct IHIC as [Za [A B]]; try eapply GetLV; eauto with len;
+      subst; simpl.
     eexists; split; eauto.
-    exploit computeParameters_AP_LV; try eapply eq; eauto with len.
-    edestruct (get_length_eq _ GetDL (eq_sym LEN1)).
-    edestruct PIR2_nth as [? [? SUB]]; try eapply H; eauto using zip_get.
-    get_functional. rewrite <- H6, <- B. cases in SUB.
-    + inv SUB.
-      (* TODO improve cset_tac *)
-      revert H5. clear_all; hnf; intros; cset_tac. eapply H1, H5. cset_tac.
-    + unfold lminus in NOTCOND.
-      revert NOTCOND; clear_all; cset_tac.
-  - edestruct get_zip as [bv [bv' [GET1 [GET2 ?]]]]; eauto; subst.
+    inv_get.
+    exploit (@computeParameters_AP_LV Lv ZL (addParam x (Lv \\ ZL) AP));
+      try eapply H2; eauto with len.
+    PIR2_inv. unfold addParam in H3. inv_get.
+    rewrite <- H7.
+    revert H9 B. clear_all; cases; intros; cset_tac.
+    idtac "improve".
+    eapply B; cset_tac.
+    eapply H3. eapply H9. cset_tac.
+    eapply B. cset_tac.
+  - inv_get.
     edestruct IHIC as [? [? SUB]]; eauto; subst.
-    destruct bv'; eexists; split; simpl; eauto.
-    + rewrite <- H7, <- SUB. clear_all; cset_tac.
-    + rewrite <- H7, <- SUB. reflexivity.
-  - edestruct get_zip as [bv [bv' [GET1 [GET2 ?]]]]; eauto; subst.
+    setoid_rewrite <- H8. setoid_rewrite <- SUB.
+    destruct x0;
+    eexists; simpl; split; eauto; clear_all; cset_tac.
+  - inv_get.
     edestruct IHIC as [? [? SUB]]; eauto; subst.
-    destruct bv; eexists; split; simpl; eauto.
-    + rewrite <- H8, <- SUB. clear_all; cset_tac.
-    + rewrite <- H8, <- SUB. reflexivity.
-  - simpl in *.
-    intros.
-    edestruct (mapi_get _ _ GetLV) as [x [ H]]; eauto; subst.
-    cases; eauto. inv_get. (*TODO this repeat should not be necc *)
+    setoid_rewrite <- H9. setoid_rewrite <- SUB.
+    destruct x;
+    eexists; simpl; split; eauto; clear_all; cset_tac.
+  - simpl in *. unfold keep in GetLV.
+    inv_get.
+    cases; eauto.
     eexists; split; eauto.
-    rewrite <- H2. eauto with cset.
-  - edestruct IHIC as [? [A B]]; eauto with len.
-    subst; simpl. eexists; split; eauto.
-    exploit computeParameters_AP_LV; try eapply eq; eauto with len.
-    edestruct (get_length_eq _ GetDL (eq_sym LEN1)).
-    edestruct PIR2_nth as [? [? SUB]]; try eapply H; eauto using zip_get.
-    get_functional. rewrite <- H7, <- B. cases in SUB.
-    + inv SUB.
-      (* TODO improve cset_tac *)
-      revert H3. clear_all; hnf; intros; cset_tac. eapply H1, H3. cset_tac.
-    + unfold lminus in NOTCOND.
-      revert NOTCOND; clear_all; cset_tac.
-  - lnorm.
-    simpl in *. inv_get.
-    edestruct (get_length_eq _ H0 H4) as [alv GETalv].
-    exploit (@computeParameters_length (snd Zs) alv); try eapply pair_eta.
-    eapply H5; eauto. instantiate (1:=tab {} ‖F‖ ++ AP); eauto with len.
-    eauto with len.
+    rewrite <- H3. eauto with cset.
+  - edestruct IHIC as [? [A B]]; try eapply GetLV; eauto with len; subst.
+    eexists; split; eauto.
+    inv_get.
+    exploit (@computeParameters_AP_LV Lv ZL (addParam x (Lv \\ ZL) AP));
+      try eapply H5; eauto with len.
+    PIR2_inv. unfold addParam in H2. inv_get.
+    rewrite <- H8.
+    revert H6 B. clear_all; cases; intros; cset_tac.
+    idtac "improve".
+    eapply B; cset_tac.
+    eapply H3. eapply H6. cset_tac.
+    eapply B. cset_tac.
+  - lnorm. inv_get.
+    exploit (@computeParameters_length (tab {} ‖F‖ ++ AP) (snd Zs) x);
+      eauto with len.
     destruct (@get_in_range _ (snd
-          (computeParameters ((getAnn ⊝ als ++ DL) \\ (fst ⊝ F ++ ZL))
-                             (fst ⊝ F ++ ZL) (tab {} ‖F‖ ++ AP) (snd Zs) alv)) (❬F❭ + n))
+          (computeParameters ((getAnn ⊝ als ++ Lv) \\ (fst ⊝ F ++ ZL))
+                             (fst ⊝ F ++ ZL) (tab {} ‖F‖ ++ AP) (snd Zs) x)) (❬F❭ + n))
       as [pF GETpF].
-    rewrite H1. eapply get_range in GetDL. rewrite app_length, map_length. omega.
-    edestruct IHIC1; try eapply GETpF; eauto using pair_eta.
-    eauto with len. eauto with len. eapply get_app_right; eauto.
+    rewrite H6. eapply get_range in GetDL. rewrite app_length, map_length. omega.
+    edestruct IHIC1; try eapply GETpF; eauto with len.
+    eapply get_app_right; eauto.
     orewrite (n + 0 = n). eauto. eapply get_app_right; eauto.
-    rewrite map_length; eauto with len. destruct H2. subst.
-    rewrite zip_app; eauto with len.
-    rewrite zip_app in GetLV; eauto with len.
-    exploit computeParameters_length as LENb; try eapply eq; eauto with len.
-    exploit (get_olist_union_A (A:=snd ⊝ computeParametersF DL ZL AP F als));
-      try eapply GETpF.
-    eapply map_get_1. eapply zip_get_eq; eauto.
-    rewrite zip_app; eauto with len.
-    eapply computeParametersF_length; eauto. rewrite live_globals_zip; eauto.
-    destruct H2 as [? [? ?]]; subst. get_functional. simpl. eexists; split; eauto.
-    edestruct (@get_in_range _ b k); try eapply GETalv.
-    rewrite LENb. rewrite app_length, map_length. omega.
+    rewrite map_length; eauto with len.
+    dcr; subst.
+    exploit (computeParameters_length (tab {} ‖F‖ ++ AP)) as LENb;
+      try eapply H3; eauto with len.
+    edestruct get_olist_union_A' as [? [? ?]]; try eapply GetLV;
+      eauto using map_get_1, zip_get.
+    eapply computeParametersF_length; eauto with len.
+    subst; simpl. eexists; split; eauto.
+    assert (k < ❬snd
+            (computeParameters ((getAnn ⊝ als ++ Lv) \\ (fst ⊝ F ++ ZL))
+                               (fst ⊝ F ++ ZL) (tab {} ‖F‖ ++ AP) t alb)❭).
+    rewrite computeParameters_length; eauto with len.
+    edestruct (get_in_range _ H7).
     edestruct IHIC2 as [? [ ? ?]];
-      try eapply eq; eauto using map_get_1, get_app with len.
-    dcr; subst. rewrite <- H9. rewrite <- H10. rewrite <- H6, <- H8.
+      try eapply g; eauto using map_get_1, get_app with len. subst.
+    rewrite <- H10. rewrite <- H13. rewrite <- H11.
     repeat rewrite minus_union.
-    unfold lminus at 3.
     assert (of_list (fst Zs) ⊆ list_union (fst ∘ of_list ⊝ F)). {
       eapply incl_list_union. eapply map_get_1; eauto. reflexivity.
     }
-    rewrite <- H2.
-    assert (x2 ⊆ list_union (oget ⊝ take ❬F❭
-           (olist_union (snd ⊝ computeParametersF DL ZL AP F als) b))). {
-      exploit (get_olist_union_b (A:=snd ⊝ computeParametersF DL ZL AP F als));
+    rewrite <- H12.
+    assert (x4 ⊆ list_union (oget ⊝ take ❬F❭
+                                  (olist_union (snd ⊝ computeParametersF F als Lv ZL AP)
+                                               (snd
+                                                  (computeParameters
+                                                     ((getAnn ⊝ als ++ Lv) \\ (fst ⊝ F ++ ZL))
+                                                     (fst ⊝ F ++ ZL) (tab {} ‖F‖ ++ AP) t alb))))). {
+      exploit (get_olist_union_b (A:=snd ⊝ computeParametersF F als Lv ZL AP));
       try eapply g.
-      eapply computeParametersF_length; eauto. rewrite live_globals_zip; eauto.
-      destruct H11; dcr.
+      eapply computeParametersF_length; eauto.
+      destruct H14; dcr.
       eapply incl_list_union. eapply map_get_1.
       eapply get_take; eauto.
-      eassumption.
+      eapply H16.
     }
-    rewrite <- H11.
+    rewrite <- H9.
+    rewrite H14.
     clear_all; cset_tac.
   - lnorm. simpl in *. inv_get.
-    rewrite zip_app in GetLV; eauto with len.
-    rewrite zip_app; eauto with len.
-    exploit computeParameters_length; eauto. eauto with len. eauto with len.
-    destruct (@get_in_range _ b (❬F❭ + n)) as [pF GETpF].
-    rewrite H, app_length, map_length. exploit (get_range GetDL). omega.
-    edestruct IHIC; eauto. eauto with len. eauto with len.
+    exploit (computeParameters_length (tab {} ‖F‖ ++ AP));
+      try eapply H1; eauto with len.
+    assert (❬F❭ + n < ❬snd
+          (computeParameters ((getAnn ⊝ als ++ Lv) \\ (fst ⊝ F ++ ZL))
+             (fst ⊝ F ++ ZL) (tab {} ‖F‖ ++ AP) t alb)❭).
+    rewrite H0, app_length, map_length. exploit (get_range GetDL). omega.
+    destruct (get_in_range _ H4) as [pF GETpF].
+    edestruct IHIC with (AP:=tab {} ‖F‖ ++ AP); eauto with len.
     eapply get_app_right; eauto using map_get_1.
     orewrite (n+0 = n); eauto.
     eapply get_app_right; eauto using map_get_1.
     rewrite map_length; eauto. dcr; subst.
-    exploit (get_olist_union_b (A:=snd ⊝ computeParametersF DL ZL AP F als));
-      try eapply GETpF.
+    edestruct (get_olist_union_b (A:=snd ⊝ computeParametersF F als Lv ZL AP))
+      as [? [? ?]]; try eapply GETpF.
     eapply computeParametersF_length; eauto.
-    rewrite live_globals_zip; eauto.
-    destruct H0; dcr; subst; simpl. get_functional.
-    eexists; split; try reflexivity. rewrite <- H7, <- H8, <- H6.
+    get_functional.
+    eexists; split; try reflexivity. rewrite <- H7, <- H8, <- H9.
     repeat rewrite minus_union.
-    unfold lminus at 3. clear_all; cset_tac.
+    clear_all; cset_tac.
 Qed.
 
-Lemma computeParameters_isCalled_get_Some DL ZL AP s lv an' LV n p A D Z
-  : computeParameters (zip lminus DL ZL) ZL AP s lv = (an', LV)
-    -> live_sound Imperative (zip pair DL ZL) s lv
-    -> length AP = length DL
-    -> length DL = length ZL
+Lemma computeParameters_isCalled_get_Some Lv ZL AP s lv n p A D Z
+  : live_sound Imperative ZL Lv s lv
+    -> length AP = length Lv
+    -> length Lv = length ZL
     -> isCalled s (LabI n)
-    -> n < ❬LV❭
-    -> get DL n D
+    -> n < ❬snd (computeParameters (Lv \\ ZL) ZL AP s lv)❭
+    -> get Lv n D
     -> get ZL n Z
-    -> get (olist_union A LV) n p
-    -> (forall (n0 : nat) (a : 〔؟⦃var⦄〕), get A n0 a -> ❬LV❭ = ❬a❭)
+    -> get (olist_union A (snd (computeParameters (Lv \\ ZL) ZL AP s lv))) n p
+    -> (forall (n0 : nat) (a : 〔؟⦃var⦄〕),
+          get A n0 a -> ❬a❭ = ❬snd (computeParameters (Lv \\ ZL) ZL AP s lv)❭)
     -> exists Za, p = Some Za /\ D \ of_list Z \ Za ⊆ (getAnn lv).
 Proof.
-  intros CPEQ LS LEN1 LEN2 IC LE GETDL GETZL GET LEN3.
-  destruct (@get_in_range _ LV n); eauto.
+  intros LS LEN1 LEN2 IC LE GETDL GETZL GET LEN3.
+  destruct (get_in_range _ LE); eauto.
   edestruct computeParameters_isCalled_Some; eauto; dcr; subst.
   edestruct get_olist_union_b; eauto; dcr.
   get_functional.
@@ -513,19 +529,14 @@ Definition ominus' (s : set var) (t : option (set var)) := mdo t' <- t; ⎣s \ t
 Definition minuso (s : set var) (t : option (set var)) := ⎣s \ oget t ⎦.
 
 Lemma zip_ominus_contra DL b b'
-  : length DL = length b
-    -> length b = length b'
-    -> PIR2 (fstNoneOrR Subset) b b'
+  : PIR2 (fstNoneOrR Subset) b b'
     -> zip ominus' DL b ≿ zip ominus' DL b'.
 Proof.
-  intros. eapply length_length_eq in H. eapply length_length_eq in H0.
-  general induction H; inv H0; simpl.
-  - reflexivity.
+  intros.
+  general induction H; destruct DL; simpl; eauto using PIR2.
   - econstructor; eauto.
-    + destruct y, y0; simpl; try now econstructor.
-      * inv H1. inv pf. econstructor. unfold flip; cset_tac; intuition.
-      * inv H1. inv pf.
-    + inv H1. eauto.
+    + inv pf; simpl; econstructor.
+      unfold flip. rewrite H0. eauto.
 Qed.
 
 Lemma restrict_zip_ominus' DL LV lv x al
@@ -667,28 +678,12 @@ Proof.
       eapply length_eq_length in LEN2. omega.
 Qed.
 
-Lemma mkGlobals_zip_ominus' (F:list (params*stmt)) als LV
-  : ❬F❭ = ❬als❭ -> ❬F❭ = ❬LV❭
-    -> PIR2 (option_eq Equal)
-           (mkGlobals F (oto_list ⊝ LV) als)
-           (minuso ⊜ ((getAnn ⊝ als) \\ (fst ⊝ F)) LV).
-Proof.
-  intros. rewrite map_zip.
-  eapply zip_ext_PIR2; eauto with len.
-  intros. inv_get.
-  unfold minuso, lminus, oto_list.
-  destruct y'.
-  - econstructor. rewrite of_list_3; eauto.
-  - econstructor; eauto.
-Qed.
-
 Lemma PIR2_ominus_minuso A B B'
-  : length A = length B
-    -> PIR2 (fstNoneOrR Subset) B B'
+  : PIR2 (fstNoneOrR Subset) B B'
     -> ominus' ⊜ A B ≿ minuso ⊜ A B'.
 Proof.
-  intros LEN EQ. length_equify.
-  general induction LEN; inv EQ; simpl; eauto.
+  intros EQ.
+  general induction EQ; destruct A; simpl; eauto.
   econstructor; eauto.
   inv pf; simpl; econstructor.
   simpl. unfold flip. rewrite H. reflexivity.
@@ -697,75 +692,225 @@ Qed.
 Hint Extern 10 (forall _ _, get (snd ⊝ computeParametersF ?DL ?ZL ?AP ?F ?als) _ _ -> ❬?LVb❭ = ❬_❭)
 => eapply computeParametersF_length : len.
 
-Lemma computeParameters_trs DL ZL AP s an' LV lv
-: live_sound Imperative (zip pair DL ZL) s lv
-  -> computeParameters (zip lminus DL ZL) ZL AP s lv = (an', LV)
-  -> noUnreachableCode s
-  -> PIR2 Subset AP (zip lminus DL ZL)
-  -> length DL = length ZL
-  -> length ZL = length AP
-  -> trs (restrict (zip ominus' (zip lminus DL ZL) LV) (getAnn lv))
-        (List.map oto_list LV)  s lv an'.
+Hint Extern 1 =>
+match goal with
+  [ |- context [ ❬snd (computeParameters _ _ _ _ _)❭ ] ] =>
+  rewrite computeParameters_length; eauto with len
+end : len.
+
+
+Lemma app_length_le_ass X (L:list X) L' k
+  : length L + length L' <= k
+    -> length (L ++ L') <= k.
 Proof.
-  intros LIVE CPEQ NOUR P LEN1 LEN2.
-  remember (zip pair DL ZL) as DLZL. revert_except LIVE.
-  induction LIVE; simpl in *; intros; (repeat let_case_eq); inv NOUR.
-  - invc CPEQ. eapply trsExp, trs_monotone_DL.
-    + eapply IHLIVE; try eapply eq; eauto 10 using addParam_Subset with len.
-    + exploit computeParameters_AP_LV; eauto with len.
-      exploit computeParameters_length; eauto with len.
-      rewrite restrict_comp_meet.
+  intros; subst. rewrite app_length; eauto.
+Qed.
+
+Lemma app_length_le_ass_right X (L:list X) L' k
+  : k <= length L + length L'
+    -> k <= length (L ++ L').
+Proof.
+  intros; subst. rewrite app_length; eauto.
+Qed.
+
+Lemma map_length_le_ass X Y (L:list X) (f:X->Y) k
+  : length L <= k
+    -> length (List.map f L) <= k.
+Proof.
+  intros; subst. rewrite map_length; eauto.
+Qed.
+
+Lemma map_length_le_ass_right X Y (L:list X) (f:X->Y) k
+  : length L = k
+    -> k = length (List.map f L).
+Proof.
+  intros; subst. rewrite map_length; eauto.
+Qed.
+
+Lemma zip_length_le_ass_right (X Y Z : Type) (f : X -> Y -> Z) (L : list X) (L' : list Y) k
+  : length L = length L'
+    -> k <= length L
+    -> k <= length (zip f L L').
+Proof.
+  intros; subst; rewrite zip_length2; eauto.
+Qed.
+
+Hint Resolve zip_length_le_ass_right : len.
+
+Hint Resolve app_length_le_ass app_length_le_ass_right map_length_le_ass map_length_le_ass_right
+  : len.
+
+Lemma take_zip (X Y Z : Type) (f : X -> Y -> Z) (L : list X) (L' : list Y) n
+  : take n (zip f L L') = zip f (take n L) (take n L').
+Proof.
+  intros. general induction n; simpl; eauto.
+  - destruct L, L'; simpl; eauto.
+    f_equal; eauto.
+Qed.
+
+Instance zip_eq_m (X Y Z : Type)
+  : Proper (eq ==> eq ==> eq ==> eq) (@zip X Y Z).
+Proof.
+  unfold Proper, respectful; intros; subst; eauto.
+Qed.
+
+Lemma take_app_eq n X (L L':list X)
+  : n = length L
+    -> take n (L ++ L') = L.
+Proof.
+  intros. subst. general induction L; simpl; eauto.
+  f_equal; eauto.
+Qed.
+
+Lemma ominus'_Some_oto_list A B C1 C2
+  : PIR2 ≼ C1 C2
+    -> ominus' ⊜ (A \\ B) C1 ≿ Some ⊝ A \\ app (A:=var) ⊜ B (oto_list ⊝ C2).
+Proof.
+  intros. general induction H; simpl; destruct A, B; try reflexivity.
+  - simpl; econstructor; eauto.
+    + inv pf; simpl ominus'. econstructor.
+      econstructor. unfold flip, oto_list.
+      rewrite of_list_app. rewrite of_list_3.
+      unfold flip in H0. rewrite <- minus_union.
+      rewrite H0. reflexivity.
+Qed.
+
+Lemma computeParameters_trs ZL Lv AP s lv
+: live_sound Imperative ZL Lv s lv
+  -> noUnreachableCode s
+  -> PIR2 Subset AP (Lv \\ ZL)
+  -> length Lv = length ZL
+  -> length ZL = length AP
+  -> trs (restrict (zip ominus' (Lv \\ ZL)
+                       (snd (computeParameters (Lv \\ ZL) ZL AP s lv))) (getAnn lv))
+                  (List.map oto_list (snd (computeParameters (Lv \\ ZL) ZL AP s lv)))
+                  s lv
+                  (fst (computeParameters (Lv \\ ZL) ZL AP s lv)).
+Proof.
+  intros LIVE NOUR P LEN1 LEN2.
+  revert_except LIVE.
+  induction LIVE; simpl in *; intros; repeat let_case_eq;
+    repeat let_pair_case_eq; inv NOUR; simpl in *.
+  - eapply trsExp, trs_monotone_DL.
+    + eapply IHLIVE; eauto 10 using addParam_Subset with len.
+    + rewrite restrict_comp_meet.
       assert (SEQ:lv ∩ (lv \ singleton x) [=] lv \ singleton x) by cset_tac.
       rewrite SEQ. eapply restrict_zip_ominus'; eauto with len.
-      eapply PIR2_not_in; eauto with len.
-  - invc CPEQ. exploit (computeParameters_length _ _ _ eq); eauto with len.
-    exploit (computeParameters_length _ _ _ eq0); eauto with len.
-    econstructor.
-    + exploit (PIR2_zip_ounion b b0); eauto with len.
-      eapply trs_monotone_DL_AP; eauto.
-      eapply restrict_subset2; eauto.
-      eapply zip_ominus_contra; eauto with len.
-    + exploit (PIR2_zip_ounion' b0 b); eauto with len.
-      eapply trs_monotone_DL_AP; eauto.
-      eapply restrict_subset2; eauto.
-      eapply zip_ominus_contra; eauto with len.
-  - invc CPEQ. edestruct get_zip as [D [L [GETZL [GETDL EQ]]]]; dcr; eauto. invc EQ.
-    edestruct (get_length_eq _ GETDL LEN2) as [ap GETAP].
-    exploit (@keep_Some _ AP (labN l)) as GETKEEP; eauto.
-    exploit (zip_get lminus GETZL GETDL) as GETLMINUS.
-    exploit (zip_get ominus' GETLMINUS GETKEEP) as GETOMINUS.
-    econstructor.
-    eapply restrict_get_Some. eapply GETOMINUS. unfold lminus.
-    rewrite <- H0. clear_all; cset_tac.
-    eapply map_get_1; eauto.
-  - invc CPEQ. econstructor.
 
-  - invc CPEQ. eapply trsExtern, trs_monotone_DL.
-    eapply IHLIVE; try eapply eq; eauto 10 using addParam_Subset with len.
-    exploit computeParameters_AP_LV; eauto with len.
-    exploit computeParameters_length; eauto with len.
-    rewrite restrict_comp_meet.
-    assert (SEQ:lv ∩ (lv \ singleton x) [=] lv \ singleton x) by cset_tac.
-    rewrite SEQ. eapply restrict_zip_ominus'; eauto with len.
-    eapply PIR2_not_in; eauto with len.
+      eapply PIR2_not_in; [ eapply computeParameters_AP_LV; eauto with len
+                          | eauto with len].
+  - econstructor.
+    + eapply trs_monotone_DL_AP; eauto.
+      eapply restrict_subset2; eauto.
+      eapply zip_ominus_contra; eauto using PIR2_zip_ounion with len.
+      eapply PIR2_zip_ounion; eauto with len.
+    + eapply trs_monotone_DL_AP; eauto using PIR2_zip_ounion' with len.
+      eapply restrict_subset2; eauto with len.
+      eapply zip_ominus_contra; eauto using PIR2_zip_ounion' with len.
+  - inv_get.
+    econstructor.
+    + eapply restrict_get_Some.
+      eapply zip_get_eq. eapply zip_get; eauto.
+      eapply keep_Some; eauto. simpl. reflexivity.
+      rewrite <- H1. eauto with cset.
+    + eapply map_get_1. eapply keep_Some; eauto.
+  - econstructor.
 
-  - rewrite <- zip_app in eq; eauto with len.
-    rewrite live_globals_zip in LIVE; eauto with len.
+  - eapply trsExtern, trs_monotone_DL.
+    + eapply IHLIVE; eauto 10 using addParam_Subset with len.
+    + rewrite restrict_comp_meet.
+      assert (SEQ:lv ∩ (lv \ singleton x) [=] lv \ singleton x) by cset_tac.
+      rewrite SEQ. eapply restrict_zip_ominus'; eauto with len.
+      eapply PIR2_not_in; [ eapply computeParameters_AP_LV; eauto with len
+                          | eauto with len].
+  - lnorm. econstructor.
+    + eauto with len.
+    + eauto with len.
+    + rewrite map_length. rewrite take_less_length; eauto.
+      rewrite zip_length2; [eauto 20 with len|].
+      rewrite fold_zip_ounion_length.
+      * rewrite computeParameters_length; eauto with len.
+      * eapply computeParametersF_length; eauto with len.
+    + intros. inv_get. simpl.
+      rewrite <- List.map_app. rewrite <- take_eta.
+      eapply trs_monotone_DL_AP.
+      * eapply H1; eauto using PIR2_Subset_tab_extend with len.
+      * { rewrite (take_eta (length F) (zip ominus' _ _)).
+          do 2 rewrite restrict_app.
+          eapply PIR2_app.
+          - rewrite restrict_disj.
+            + eapply restrict_subset2; eauto.
+              do 2 rewrite take_zip.
+              rewrite take_app_eq; [|eauto with len].
+              rewrite take_app_eq; [|eauto with len].
+              eapply ominus'_Some_oto_list.
+              eapply PIR2_take. eapply PIR2_addAdds'.
+              eauto with len.
+              eapply PIR2_combineParams_get;
+                [ eapply computeParametersF_length_pair; eauto with len
+                | eauto with len
+                | eapply zip_get; eauto
+                | reflexivity ].
+            + intros.
+              inv_get.
+
+          - rewrite restrict_comp_meet.
+            assert (lvsEQ:getAnn lvs \ of_list (fst Zs ++ oto_list x)
+                                 [=] lv ∩ (getAnn lvs \ of_list (fst Zs ++ oto_list x))).         {
+              edestruct (@get_in_range _ LVb n). omega.
+              subst NPL. inv_get.
+              eapply get_in_range_app in H12; eauto with len.
+              inv_get.
+              edestruct computeParameters_isCalled_get_Some; try eapply eq;
+                eauto using get_app, map_get_1 with len. dcr; subst.
+              simpl. unfold lminus. rewrite H3 in H13.
+              rewrite of_list_app. repeat rewrite of_list_3.
+              revert H13; clear_all; cset_tac.
+              eapply H13. cset_tac.
+            }
+
+        }
+
+      * eapply PIR2_addAdds'; eauto with len.
+        eapply PIR2_combineParams_get; [ | | | reflexivity].
+        eapply computeParametersF_length_pair; eauto with len.
+        eauto with len. eapply zip_get_eq; eauto.
+    + rewrite <- List.map_app. rewrite <- take_eta.
+      eapply trs_monotone_DL_AP.
+      eapply IHLIVE; eauto using PIR2_Subset_tab_extend with len.
+      * { rewrite (take_eta (length F) (zip ominus' _ _)).
+          rewrite restrict_app.
+          eapply PIR2_app.
+          - eapply PIR2_restrict.
+            do 2 rewrite take_zip.
+            rewrite take_app_eq; [|eauto with len].
+            rewrite take_app_eq; [|eauto with len].
+            eapply ominus'_Some_oto_list.
+            eapply PIR2_take. eapply PIR2_addAdds'.
+            eauto with len.
+            eapply PIR2_combineParams; [| reflexivity].
+            eapply computeParametersF_length_pair; eauto with len.
+          - eapply restrict_subset2; eauto.
+            rewrite drop_zip; [|eauto with len].
+            rewrite drop_zip; [|eauto with len].
+            repeat (rewrite drop_length_ass; [| eauto with len]).
+            eapply zip_ominus_contra.
+            eapply PIR2_drop; eauto.
+            eapply PIR2_addAdds'. eauto with len.
+            eapply PIR2_combineParams; [| reflexivity].
+            eapply computeParametersF_length_pair; eauto with len.
+        }
+      * eapply PIR2_addAdds'; eauto with len.
+        eapply PIR2_combineParams; [|reflexivity].
+        eapply computeParametersF_length_pair; eauto with len.
+Qed.
+
+
     rename b0 into LVb.
     exploit (computeParameters_length _ _ _ eq) as LENLVb; eauto with len.
     exploit (computeParameters_LV_DL _ _ LIVE eq) as PIRLVb;
       eauto using PIR2_Subset_tab_extend with len.
     invc CPEQ.
-    set (NP:=list_union (oget
-                           ⊝ take ❬F❭
-                           (olist_union (snd
-                                           ⊝
-                                           computeParametersF DL ZL
-                                           AP F als) LVb))
-                        ∪ list_union (fst ∘ of_list ⊝ F)).
-    set (NPL:=(addAdd NP
-                      ⊜ ((getAnn ⊝ als) \\ (fst ⊝ F) ++ DL \\ ZL)
-                      (olist_union (snd ⊝ computeParametersF DL ZL AP F als) LVb))).
     assert (LENcPF:forall n aa, get (computeParametersF DL ZL AP F als) n aa -> ❬snd aa❭ = ❬LVb❭).
     {
       intros n aa GET. destruct aa as [an LV]. inv_get.
@@ -851,7 +996,7 @@ Proof.
         eapply PIR2_take; eauto.
 
         intros. inv_get.
-        unfold lminus, oto_list.
+        unfold oto_list.
         subst NPL. inv_get.
         eapply get_in_range_app in H11; eauto with len.
         eapply get_in_range_app in H13; eauto with len.
@@ -864,7 +1009,7 @@ Proof.
           eauto using get_app, map_get_1 with len. dcr; subst.
         Opaque to_list.
         simpl in *. rewrite of_list_app.
-        repeat rewrite of_list_3. unfold lminus.
+        repeat rewrite of_list_3.
         rewrite minus_union.
         eapply disj_minus.
         rewrite (meet_comm _ (getAnn lvs)) at 1.
